pulse/examples/steel/arraystructs/IntOrBool.fst
@@ -1,0 +1,61 @@
+module IntOrBool
+
+open AggregateRef
+open FStar.PCM
+open FStar.PCM.Extras
+open FStar.PCM.POD
+open Steel.Effect
+module M = Steel.Memory
+module A = Steel.Effect.Atomic
+
+type int_or_bool_case = | I | B
+let int_or_bool_cases k = match k with
+  | I -> pod int
+  | B -> pod bool
+let int_or_bool = union int_or_bool_cases
+
+let int_or_bool_cases_pcm k : refined_one_pcm (int_or_bool_cases k) = match k with
+  | I -> pod_pcm int
+  | B -> pod_pcm bool
+let int_or_bool_pcm = union_pcm int_or_bool_cases_pcm
+
+let mk_int i = Some (|I, Ghost.reveal i|)
+let mk_bool b = Some (|B, Ghost.reveal b|)
+
+let re_i = case_refinement int_or_bool_cases_pcm I
+let re_b = case_refinement int_or_bool_cases_pcm B
+
+/// Lenses for cases
+
+let _i = case int_or_bool_cases_pcm I
+let _b = case int_or_bool_cases_pcm B
+
+/// Taking pointers to the i and b cases of an int_or_bool
+
+let addr_of_i (#i: Ghost.erased (pod int)) (p: ref 'a int_or_bool_pcm)
+: SteelT (q:ref 'a (pod_pcm int){q == ref_focus (ref_refine p re_i) _i})
+    (p `pts_to` mk_int i)
+    (fun q -> q `pts_to` i)
+= let mk_int_i : Ghost.erased (refine_t (refinement_f re_i)) = Some (|I, Ghost.reveal i|) in
+  A.change_equal_slprop (p `pts_to` mk_int i) (p `pts_to` Ghost.reveal mk_int_i);
+  addr_of_union_lens p _i (Ghost.reveal mk_int_i)
+
+let unaddr_of_i (#i: Ghost.erased (pod int)) (#opened: M.inames)
+  (p: ref 'a int_or_bool_pcm)
+  (q: ref 'a (pod_pcm int){q == ref_focus (ref_refine p re_i) _i})
+: A.SteelGhostT unit opened (q `pts_to` i) (fun _ -> p `pts_to` mk_int i)
+= unaddr_of_union_lens q p _i i
+
+let addr_of_b (#b: Ghost.erased (pod bool)) (p: ref 'a int_or_bool_pcm)
+: SteelT (q:ref 'a (pod_pcm bool){q == ref_focus (ref_refine p re_b) _b})
+    (p `pts_to` mk_bool b)
+    (fun q -> q `pts_to` b)
+= let mk_bool_b : Ghost.erased (refine_t (refinement_f re_b)) = Some (|B, Ghost.reveal b|) in
+  A.change_equal_slprop (p `pts_to` mk_bool b) (p `pts_to` Ghost.reveal mk_bool_b);
+  addr_of_union_lens p _b (Ghost.reveal mk_bool_b)
+
+let unaddr_of_b (#b: Ghost.erased (pod bool)) (#opened: M.inames)
+  (p: ref 'a int_or_bool_pcm)
+  (q: ref 'a (pod_pcm bool){q == ref_focus (ref_refine p re_b) _b})
+: A.SteelGhostT unit opened (q `pts_to` b) (fun _ -> p `pts_to` mk_bool b)
+= unaddr_of_union_lens q p _b b
